Trees234.thy
@@ -1,0 +1,5 @@
+theory Trees234
+imports "HOL-Data_Structures.Tree234_Set"
+begin
+
+end
